Examples/hashtab.v
@@ -1,7 +1,8 @@
-From mathcomp Require Import ssreflect ssrbool ssrnat eqtype ssrfun seq fintype tuple finfun finset.
+From Coq Require Import ssreflect ssrbool ssrfun.
+From mathcomp Require Import ssrnat eqtype seq fintype tuple finfun finset.
 From fcsl Require Import axioms prelude pred ordtype finmap.
 From fcsl Require Import pcm unionmap heap.
-From HTT Require Import domain model heapauto.
+From HTT Require Import model heapauto.
 From HTT Require Import array kvmaps.
 Set Implicit Arguments.
 Unset Strict Implicit.
@@ -11,62 +12,94 @@ Obligation Tactic := auto.
 Module HashTab.
 Section HashTab.
 
+(* a hash table is an array of buckets, i.e. KV maps *)
+(* bucket indices are provided by the hash function *)
+
 Variables (K : ordType) (V : Type) (buckets : KVmap.Sig K V)
           (n : nat) (hash : K -> 'I_n).
 Definition hashtab := {array 'I_n -> KVmap.tp buckets}.
 Notation KVshape := (@KVmap.shape _ _ buckets).
 Notation table := (table KVshape).
+Notation nil := (nil K V).
 
 (* TODO is there another way to prevent unfolding these? *)
 Opaque Array.write Array.new Array.free Array.read.
 
-Definition shape x s :=
-  [Pred h | exists tab bucket,
-           [/\ forall k, fnd k s = fnd k (bucket (hash k)),
-               forall i k, k \in supp (bucket i) -> hash k = i &
-               h \In Array.shape x tab # sepit setT (table tab bucket)] ].
+Check Array.new.
 
+(* hash table is specified by a single finMap *)
+(* which is morally a "flattening" of all buckets *)
+Definition shape x (s : finMap K V) :=
+  [Pred h | exists (tab : {ffun 'I_n -> KVmap.tp buckets})   (* array spec *)
+                   (bucket : 'I_n -> finMap K V),            (* buckets spec *)
+            [/\ forall k, fnd k s = fnd k (bucket (hash k)),
+                forall i k, k \in supp (bucket i) -> hash k = i &
+                h \In Array.shape x tab # sepit setT (table tab bucket)] ].
+
+(* new hash map is an array of `n` empty buckets *)
+
+(* bucket initialization loop invariant: *)
+(* at iteration k, the heap holds the array and k empty buckets *)
 Definition new_loopinv x := forall k,
   STsep (fun h => k <= n /\ exists tab,
            h \In Array.shape x tab #
-                   sepit [set x:'I_n | x < k] (table tab (fun => nil K V)),
-         [vfun y => shape y (nil K V)]).
+                   sepit [set x:'I_n | x < k] (table tab (fun=> nil)),
+         [vfun y => shape y nil]).
 
-Program Definition new : STsep (emp, [vfun y => shape y (nil K V)]) :=
+Program Definition new : STsep (emp, [vfun y => shape y nil]) :=
   Do (t <-- Array.new _ (KVmap.default buckets);
-      Fix (fun (loop : new_loopinv t) k =>
+      let go := Fix (fun (loop : new_loopinv t) k =>
            Do (if decP (b := k < n) idP is left pf then
                  b <-- KVmap.new buckets;
                  Array.write t (Ordinal pf) b;;
                  loop k.+1
-               else ret t)) 0).
+               else ret t))
+      in go 0).
+(* first the bucket initialization loop *)
 Next Obligation.
+(* pull out preconditions, branch on k comparison *)
 move=>/= arr loop k [] _ /= [Eleq][tab][h1][h2][-> H1]; case: decP; last first.
-- case: ltnP Eleq (eqn_leq k n)=>// _ -> /= /eqP Ek _ H.
-  step=>_.
-  exists tab, (fun _:'I_n => nil K V); split=>//; exists h1, h2; do!split=>//.
-  apply/tableP2: H=>//= x.
-  by rewrite Ek !in_set ltn_ord.
-move=>Ho H2; rewrite -[h1 \+ h2]unitL.
+- (* k = n, return the array pointer *)
+  case: ltnP Eleq (eqn_leq k n)=>// _ -> /= /eqP Ek _ H; step=>_.
+  (* pass through the constructed table, aggregated finmap is empty *)
+  exists tab, (fun _:'I_n => nil); split=>//; exists h1, h2; split=>//.
+  (* h2 holds the table *)
+  by apply/tableP2: H=>//= x; rewrite Ek !in_set ltn_ord.
+(* k < n *)
+move=>pf H2; rewrite -[h1 \+ h2]unitL.
+(* allocate an empty bucket *)
 apply/[stepR] @ Unit=>//= b m Hm.
+(* write its id to the array under index k *)
 apply/[stepR tab] @ h1=>{H1}//= [[]] m2 [E2 V2].
+(* invoke the loop *)
 apply/[gE]=>//=; split=>//; rewrite joinCA.
-exists [ffun z => if z == Ordinal Ho then b else tab z], m2, (m \+ h2); split=>//.
-rewrite (sepitS (Ordinal Ho)) in_set leqnn {1}/table ffunE eq_refl.
-exists m, h2; do!split=>//.
+(* extend the table by the new index/bucket pair, simplify *)
+exists [ffun z => if z == Ordinal pf then b else tab z], m2, (m \+ h2); split=>//{m2 E2 V2}.
+(* remove the new bucket from the heap *)
+rewrite (sepitS (Ordinal pf)) in_set leqnn {1}/table ffunE eq_refl; exists m, h2; do!split=>//.
 apply: tableP2 H2=>//.
 - by case=>x ?; rewrite !in_set -val_eqE /= ltnS (leq_eqVlt x); case: ltngtP.
+(* removing k from the domain of the new table gives the old table back *)
 by move=>x _; rewrite in_set ffunE; case: eqP=>//->; rewrite ltnn.
 Qed.
+(* now the outer function *)
 Next Obligation.
-move=>/= [] ? ->.
+(* simplify *)
+move=>/= [] _ ->.
+(* allocate the array *)
 apply: [stepE]=>//=; case=>//= y m [H Vm].
+(* invoke the loop with index 0 *)
 apply: [gE]=>//=; split=>//.
-exists [ffun => KVmap.default buckets], m, Unit.
-do!split=>//=; first by rewrite unitR.
+(* the table is empty *)
+exists [ffun => KVmap.default buckets], m, Unit; split=>//=; first by rewrite unitR.
+(* there are no bucket in the heap yet *)
 by rewrite (eq_sepit (s2 := set0)) // sepit0.
 Qed.
 
+(* freeing a hashtable is freeing the array + buckets *)
+
+(* loop invariant: *)
+(* at iteration k, the heap still holds the array and n-k buckets *)
 Definition free_loopinv x := forall k,
   STsep (fun h => k <= n /\ exists t b,
           h \In Array.shape x t #
@@ -75,33 +108,48 @@ Definition free_loopinv x := forall k,
 
 Program Definition free x : {s}, STsep (shape x s,
                                         [vfun _ : unit => emp]) :=
+  (* we add an extra Do here so we can derive the precondition from the loop *)
   Do (Fix (fun (loop : free_loopinv x) k =>
           Do (if decP (b := k < n) idP is left pf then
                 b <-- Array.read x (Ordinal pf);
                 KVmap.free b;;
                 loop k.+1
                else Array.free x)) 0).
+(* first the loop *)
 Next Obligation.
+(* pull out the ghost + preconditions, branch on k comparison *)
 move=>/= x loop k [] _ /= [Eleq][tf][bf][h1][h2][-> [H1 H2]]; case: decP; last first.
-- case: ltnP Eleq (eqn_leq k n)=>// _ -> /= /eqP Ek _ H.
-  apply: [gE]=>//=; exists tf; move: H.
-  rewrite (eq_sepit (s2 := set0)); first by rewrite sepit0=>->; rewrite unitR.
+- (* k = n *)
+  case: ltnP Eleq (eqn_leq k n)=>// _ -> /= /eqP Ek _ H.
+  (* free the array *)
+  apply: [gE]=>//=; exists tf.
+  (* h2 is empty *)
+  move: H; rewrite (eq_sepit (s2 := set0)); first by rewrite sepit0=>->; rewrite unitR.
   by move=>y; rewrite Ek in_set in_set0 leqNgt ltn_ord.
+(* k < n, read from array *)
 move=>pf H; apply/[stepR tf, h1] @ h1=>//= _ _ [->->].
-move: H; rewrite (sepitS (Ordinal pf)) in_set leqnn /table.
-case=>h3[h4][{h2}-> H3 H4].
+(* split out the the k-th bucket *)
+move: H; rewrite (sepitS (Ordinal pf)) in_set leqnn; case=>h3[h4][{h2}-> H3 H4].
+(* free it *)
 apply/[stepR (bf (Ordinal pf))] @ h3=>//= [[]] _ ->; rewrite unitL.
+(* invoke loop, simplify *)
 apply: [gE]=>//=; split=>//; exists tf, bf, h1, h4; split=>//.
+(* drop the k-th entry from the table *)
 apply/tableP2/H4=>//.
 move=>z; rewrite !in_set; case: eqP=>/=.
 - by move=>->/=; rewrite ltnn.
 by move/eqP; rewrite -val_eqE /=; case: ltngtP.
 Qed.
 Next Obligation.
+(* pull out ghost+preconditions *)
 move=>/= x [fm][] h /= [tf][bf][_ _ H].
-apply: [gE]=>//=; split=>//.
-by exists tf, bf.
+(* invoke the loop, simplify *)
+by apply: [gE]=>//=; split=>//; exists tf, bf.
 Qed.
+
+(* inserting into a hashmap is inserting into corresponding bucket + updating the array *)
+(* returning the pointer is technically not needed, as the array is not moved *)
+(* but we need to fit the KV map API *)
 
 Program Definition insert x k v : {s}, STsep (shape x s,
                                               [vfun y => shape y (ins k v s)]) :=
@@ -111,25 +159,38 @@ Program Definition insert x k v : {s}, STsep (shape x s,
       Array.write x hk b';;
       ret x).
 Next Obligation.
+(* pull out ghost + deconstruct precondition *)
 move=>/= x k v [fm][] _ /= [tf][bf][Hf Hh [h1][h2][-> [/= H1 _] H2]].
+(* read the bucket from array *)
 apply/[stepR tf, h1] @ h1=>//= _ _ [->->].
+(* split out the bucket in the heap *)
 move: H2; rewrite (sepitT1 (hash k)) /table; case=>h3[h4][{h2}-> H3 H4].
+(* insert into the bucket *)
 apply/[stepR (bf (hash k))] @ h3=>//= b' m2 H'.
-apply/[stepR tf] @ h1=>{H1}//= [[]] m3 [E3 V3].
-step=>_.
+(* write the bucket to the array, return the pointer *)
+apply/[stepR tf] @ h1=>{H1}//= [[]] m3 [E3 V3]; step=>_.
+(* update the array and buckets' specs *)
 exists [ffun z => if z == hash k then b' else tf z],
        (fun b => if b == hash k then ins k v (bf b) else bf b); split=>/=.
-- move=>k0; rewrite fnd_ins; case: eqP.
-  - by move=>->; rewrite eq_refl fnd_ins eq_refl.
-  move/eqP=>Ek; case: ifP=>? //.
-  by rewrite fnd_ins (negbTE Ek).
-- move=>i0 k0; case: eqP; last by move=>_; apply: Hh.
+- (* the new buckets spec is still a flattening *)
+  move=>k0; rewrite fnd_ins; case: eqP=>[->|/eqP Ek].
+  - (* if the bucket was touched, we get the same value *)
+    by rewrite eq_refl fnd_ins eq_refl.
+  (* if not, we get the old spec back *)
+  by case: ifP=>_ //; rewrite fnd_ins (negbTE Ek).
+- (* the new buckets spec respects the hash *)
+  move=>i0 k0; case: eqP; last by move=>_; apply: Hh.
   by move=>->; rewrite supp_ins inE=>/orP; case; [move/eqP=>->|apply: Hh].
-exists m3, (m2 \+ h4); do!split=>//.
-rewrite (sepitT1 (hash k)) /table /= ffunE eq_refl.
-exists m2, h4; do!split=>//.
-by apply/tableP/H4=>/= x0; rewrite !in_set andbT ?ffunE; move/negbTE=>->.
+(* the shape is respected: first, the array fits *)
+exists m3, (m2 \+ h4); split=>//.
+(* split out the modified bucket *)
+rewrite (sepitT1 (hash k)) /table /= ffunE eq_refl; exists m2, h4; split=>//.
+(* the table fits too *)
+by apply/tableP/H4=>/= x0; rewrite !in_set andbT ?ffunE =>/negbTE->.
 Qed.
+
+(* removing from a hashmap is removing from corresponding bucket + updating the array *)
+(* returning the pointer is again not needed except for the API fit *)
 
 Program Definition remove x k :
   {s}, STsep (shape x s,
@@ -140,25 +201,37 @@ Program Definition remove x k :
       Array.write x hk b';;
       ret x).
 Next Obligation.
+(* pull out ghost + destructure precondition *)
 move=>/= x k [fm][] _ /= [tf][bf][Hf Hh [h1][h2][-> [/= H1 _] H2]].
+(* read the bucket from array *)
 apply/[stepR tf, h1] @ h1=>//= _ _ [->->].
-move: H2; rewrite (sepitT1 (hash k)) /table; case=>h3[h4][{h2}-> H3 H4].
+(* split out the bucket in the heap *)
+move: H2; rewrite (sepitT1 (hash k)); case=>h3[h4][{h2}-> H3 H4].
+(* insert into the bucket *)
 apply/[stepR (bf (hash k))] @ h3=>//= b' m2 H'.
-apply/[stepR tf] @ h1=>{H1}//= [[]] m3 [E3 V3].
-step=>_.
+(* write the bucket to the array, return the pointer *)
+apply/[stepR tf] @ h1=>{H1}//= [[]] m3 [E3 V3]; step=>_.
+(* update the array and buckets' specs *)
 exists [ffun z => if z == hash k then b' else tf z],
        (fun b => if b == hash k then rem k (bf b) else bf b); split=>/=.
-- move=>k0; rewrite fnd_rem; case: eqP.
-  - by move=>->; rewrite eq_refl fnd_rem eq_refl.
-  move/eqP=>Ek; case: ifP=>? //.
-  by rewrite fnd_rem (negbTE Ek).
-- move=>i0 k0; case: eqP; last by move=>_; apply: Hh.
+- (* the new buckets spec is still a flattening *)
+  move=>k0; rewrite fnd_rem; case: eqP.
+  - (* if the bucket was touched, the value is gone *)
+    by move=>->; rewrite eq_refl fnd_rem eq_refl.
+  (* if not, we get the old spec back *)
+  by move/eqP=>Ek; case: ifP=>_ //; rewrite fnd_rem (negbTE Ek).
+- (* the new buckets spec respects the hash *)
+  move=>i0 k0; case: eqP; last by move=>_; apply: Hh.
   by move=>->; rewrite supp_rem !inE=>/andP [] _; apply: Hh.
-exists m3, (m2\+ h4); do!split=>//.
-rewrite (sepitT1 (hash k)) /table /= ffunE eq_refl.
-exists m2, h4; do!split=>//.
-by apply/tableP/H4=>/= x0; rewrite !in_set andbT ?ffunE; move/negbTE=>->.
+(* the shape is respected: first, the array fits *)
+exists m3, (m2\+ h4); split=>//.
+(* split out the modified bucket *)
+rewrite (sepitT1 (hash k)) /table /= ffunE eq_refl; exists m2, h4; split=>//.
+(* the table fits too *)
+by apply/tableP/H4=>/= x0; rewrite !in_set andbT ?ffunE =>/negbTE->.
 Qed.
+
+(* looking up in a hashmap is looking up in the corresponging bucket *)
 
 Program Definition lookup x k :
   {s}, STsep (shape x s,
@@ -166,13 +239,21 @@ Program Definition lookup x k :
   Do (b <-- Array.read x (hash k);
       KVmap.lookup b k).
 Next Obligation.
+(* pull out ghost + destructure precondition *)
 move=>/= x k [fm][] _ /= [tf][bf][Hf Hh [h1][h2][-> H1 H2]].
+(* read the bucket from array *)
 apply/[stepR tf, h1] @ h1=>//= _ _ [->->].
-move: H2; rewrite (sepitT1 (hash k)) /table; case=>h3[h4][{h2}-> H3 H4].
+(* split out the bucket in the heap *)
+move: H2; rewrite (sepitT1 (hash k)); case=>h3[h4][{h2}-> H3 H4].
+(* look up in the bucket, simplify *)
 apply/[gR (bf (hash k))] @ h3=>//= r m2 [H2 Hr] _; split; last by rewrite Hf.
+(* the shape is preserved, as nothing was modified *)
 exists tf, bf; split=>//=; exists h1, (m2 \+ h4); split=>//.
-by rewrite (sepitT1 (hash k)) /table; exists m2, h4.
+by rewrite (sepitT1 (hash k)); vauto.
 Qed.
+
+
+(* hash table is a KV map *)
 
 Definition HashTab := KVmap.make (Array null) new free insert remove lookup.
 
