Examples/kvmaps.v
@@ -6,20 +6,22 @@ From Coq Require Import ssreflect ssrbool ssrfun.
 From mathcomp Require Import eqtype seq path.
 From fcsl Require Import axioms pred ordtype finmap.
 From fcsl Require Import pcm unionmap heap automap.
-From HTT Require Import interlude domain model heapauto.
+From HTT Require Import interlude model heapauto.
 Set Implicit Arguments.
 Unset Strict Implicit.
 Unset Printing Implicit Defensive.
 Obligation Tactic := auto.
 
-(********************)
-(* stateful KV maps *)
-(********************)
+(***********************)
+(* stateful KV map ADT *)
+(***********************)
 
 Module KVmap.
 Record Sig (K : ordType) (V : Type) : Type :=
   make {tp :> Type;
+
         default : tp;
+
         shape : tp -> {finMap K -> V} -> Pred heap;
 
         new : STsep (emp, [vfun x => shape x (nil K V)]);
@@ -40,9 +42,9 @@ Record Sig (K : ordType) (V : Type) : Type :=
                                [vfun y m => m \In shape x s /\ y = fnd k s])}.
 End KVmap.
 
-(**************************************************)
-(* KVmap implemented as a sorted association list *)
-(**************************************************)
+(**********************************************************)
+(* KV map implemented as a sorted association linked list *)
+(**********************************************************)
 
 Module AssocList.
 Section AssocList.
@@ -51,26 +53,27 @@ Variable (K : ordType) (V : Set).
 Notation fmap := (finMap K V).
 Notation nil := (nil K V).
 
-(* Data is stored in a sorted associative linked list. *)
-
+(* single entry of the map as a triple of heap cells *)
 Definition entry (p q : ptr) (k : K) (v : V) : heap :=
-  p :-> k \+ (p.+1 :-> v \+ p.+2 :-> q).
+  p :-> k \+ p.+1 :-> v \+ p.+2 :-> q.
+
+(* similarly to plain linked list, we with a generic definition of a segment and *)
+(* then specialize it to self-contained lists specified by a finMap structure *)
 
 Fixpoint shape_seg' (x y : ptr) (xs : seq (K * V)) : Pred heap :=
   if xs is (k,v) :: tl then
      [Pred h | exists q h',
-       h = x :-> k \+ (x.+1 :-> v \+ (x.+2 :-> q \+ h'))
+       h = entry x q k v \+ h'
      /\ h' \In shape_seg' q y tl]
   else [Pred h | x = y /\ h = Unit].
 
-Definition shape_seg (x y : ptr) (s : finMap K V) : Pred heap :=
+Definition shape_seg (x y : ptr) (s : fmap) : Pred heap :=
   shape_seg' x y (seq_of s).
 
-Definition shape' (x : ptr) (xs : seq (K * V)) : Pred heap :=
-  shape_seg' x null xs.
-
-Definition shape (x : ptr) (s : finMap K V) : Pred heap :=
+Definition shape (x : ptr) (s : fmap) : Pred heap :=
   shape_seg x null s.
+
+(* null pointer represents an empty map *)
 
 Lemma shape_null (s : fmap) h :
   valid h -> h \In shape null s ->
@@ -79,16 +82,19 @@ Proof.
 move=>D; case: s; case=>/=.
 - by move=>? [_ ->] //; rewrite fmapE.
 move=>[??]??[?][?][H].
-by rewrite H validPtUn in D.
+by rewrite H -!joinA validPtUn in D.
 Qed.
+
+(* non-empty well-formed region represents a non-empty map such that *)
+(* a head entry respecting the key order can be pulled out of the map *)
 
 Lemma shape_cont (s : fmap) p h :
   p != null -> h \In shape p s ->
   exists k v q h',
-   [/\ s = ins k v (behd s),            (* k:->v is the head entry*)
+   [/\ s = ins k v (behd s),            (* k:->v is the head entry *)
        all (ord k) (supp (behd s)),
-       h = p :-> k \+ (p.+1 :-> v \+ (p.+2 :-> q \+ h'))
-     & h' \In shape q (behd s)].
+       h = entry p q k v \+ h' &
+       h' \In shape q (behd s)].
 Proof.
 move=>E; case: s=>xs srt /=.
 elim: xs srt=>/=.
@@ -102,15 +108,19 @@ Qed.
 Lemma all_path (s : fmap) k : all (ord k) (supp s) -> path ord k (supp s).
 Proof. by rewrite path_sortedE // =>->/=; case: s. Qed.
 
+(* inserting an entry with minimal key is prepending to the list *)
+
 Lemma shape_cons (s : fmap) p q h k v :
    all (ord k) (supp s) -> h \In shape q s ->
-   (p :-> k \+ (p.+1 :-> v \+ (p.+2 :-> q \+ h))) \In shape p (ins k v s).
+   entry p q k v \+ h \In shape p (ins k v s).
 Proof.
 move/all_path=>S H.
 suff: ins k v s = @FinMap _ _ ((k,v)::seq_of s) S by move=>->; exists q,h.
 rewrite fmapE /=; case: s {H}S=>/= xs ??.
 by rewrite last_ins'.
 Qed.
+
+(* inserting an entry with maximal key is appending to the list *)
 
 Lemma shape_seg_rcons (s : fmap) x p q h k v :
   (* conceptually last s < k *)
@@ -128,6 +138,8 @@ exists x0, (h' \+ entry p q k v); rewrite -!joinA; split=>//.
 by apply: IH=>//; apply: (path_sorted S).
 Qed.
 
+(* disjoint maps can be concatenated if the order is respected *)
+
 Lemma shape_fcat s1 s2 h1 h2 x y :
   (* conceptually last s1 < head s2 *)
   allrel ord (supp s1) (supp s2) ->
@@ -138,43 +150,51 @@ move=>O1 H1.
 case: s2 O1=>xs; elim: xs h1 y h2 s1 H1=>/=.
 - by move=>???? H1 ? _ [Eq ->]; rewrite Eq in H1; rewrite unitR.
 move=>[k' v'] xs; rewrite /fcat /= => IH /= h1 y h2 s1 H1 srt O2 H2.
-case: H2=>z[h'][-> H']; rewrite !joinA.
-apply: IH; first 1 last.
+case: H2=>z[h'][-> H']; rewrite joinA; apply: IH; first 1 last.
 - by apply/path_sorted/srt.
 - move=>H0; rewrite (allrel_in_l (xs':=k'::supp s1) _); last by apply: supp_ins.
   rewrite allrel_consl path_all //=.
   by apply/allrel_sub_r/O2=>?; rewrite inE orbC=>->.
 - by move=>?; apply: H'.
-rewrite -!joinA; apply shape_seg_rcons=>//.
+apply: shape_seg_rcons=>//.
 by move: O2; rewrite allrel_consr =>/andP [].
 Qed.
 
 (* main procedures *)
 
+(* a new map is just a null pointer *)
+
 Program Definition new : STsep (emp, [vfun x => shape x nil]) :=
   Do (ret null).
 Next Obligation. by move=>[] /= _ ->; step. Qed.
+
+(* freeing a map is deallocating all its elements *)
 
 Definition freeT : Type :=
   forall p, {fm}, STsep (shape p fm, [vfun _ : unit => emp]).
 
 Program Definition free : freeT :=
-  Fix (fun (go : freeT) p =>
+  Fix (fun (loop : freeT) p =>
        Do (if p == null then ret tt
            else pnext <-- !(p.+2);
                 dealloc p;;
                 dealloc (p.+1);;
                 dealloc (p.+2);;
-                go pnext)).
+                loop pnext)).
 Next Obligation.
-move=>go p [fm][] i /= H; apply: vrfV=>D.
-case: eqP.
-- move=>E; step=>_; rewrite E in H.
-  by case: (shape_null D H).
-move/eqP=>E; case: (shape_cont E H)=>k[v][q][h'][_ _ -> H2].
+(* pull out ghost var, precondition, branch *)
+move=>loop p [fm][] i /= H; case: eqP=>[|/eqP] E.
+- (* reached the end, heap must be empty *)
+  by apply: vrfV=>D; step=>_; rewrite E in H; case: (shape_null D H).
+(* pull out the head entry *)
+case: (shape_cont E H)=>k[v][q][h][_ _ {i H}-> H].
+(* deallocate it *)
 do 4!step; rewrite !unitL.
+(* invoke the loop on the tail *)
 by apply: [gE (behd fm)].
 Qed.
+
+(* looking up an element in the map *)
 
 Definition lookupT k : Type :=
   forall p, {fm}, STsep (shape p fm,
@@ -182,8 +202,8 @@ Definition lookupT k : Type :=
 
 Program Definition lookup x (k : K) :
   {fm}, STsep (shape x fm,
-        [vfun y m => m \In shape x fm /\ y = fnd k fm]) :=
-  Fix (fun (go : lookupT k) (cur : ptr) =>
+              [vfun y m => m \In shape x fm /\ y = fnd k fm]) :=
+  Fix (fun (loop : lookupT k) (cur : ptr) =>
        Do (if cur == null then ret None
            else
              k' <-- !cur;
@@ -192,29 +212,39 @@ Program Definition lookup x (k : K) :
                     ret (Some v)
                else if ord k' k
                  then next <-- !(cur.+2);
-                      go next
+                      loop next
                  else ret None)) x.
 Next Obligation.
-move=>_ k go cur [fm][] h /= H; apply: vrfV=>Vh.
-case: eqP.
-- move=>Ec; step=>_; rewrite Ec in H.
-  by case: (shape_null Vh H)=>->.
-move/eqP=>Ec; case: (shape_cont Ec H)=>k'[v][next][h'][Ef O' Ei H'].
-rewrite {Vh}Ei in H *; step; case: eqP.
-- move=>Ek; do 2!step; move=>_; split=>//.
-  by rewrite Ef fnd_ins Ek eq_refl.
-move/eqP=>Ek; case: ifP=>Ho'.
-- step.
-  apply/[gR (behd fm)] @ h'=>//= v0 h0' [??] _.
-  rewrite Ef; split; first by apply: shape_cons.
-  by rewrite fnd_ins (negbTE Ek).
-move: (semiconnex Ek); rewrite {}Ho' orbC /= =>Ho'.
-step=>_; split=>//.
-apply/esym/fnd_supp.
-rewrite Ef supp_ins inE negb_or; apply/andP; split=>//.
+(* pull out ghost var+precondition, branch on cur being null *)
+move=>_ k go cur [fm][] h /= H; case: eqP=>[|/eqP] Ec.
+- (* reached the end, the heap and the spec must be empty, element not found *)
+  by apply: vrfV=>Vh; step=>_; rewrite Ec in H; case: (shape_null Vh H)=>->.
+(* pull out the head entry *)
+case: (shape_cont Ec H)=>k'[v][next][h'][Ef O' Ei H']; rewrite {h}Ei in H *.
+(* read the head key, branch on equality comparison *)
+step; case: eqP=>[|/eqP] Ek.
+- (* the key matches, return the head value *)
+  by do 2![step]=>_; split=>//; rewrite Ef fnd_ins Ek eq_refl.
+(* branch on comparison *)
+case: ifP=>Ho'.
+- (* head key is less than the needed one, loop on tail *)
+  step; apply/[gR (behd fm)] @ h'=>//= v0 h0' [H0 E0] _.
+  by rewrite Ef fnd_ins (negbTE Ek); split=>//; exact: shape_cons.
+(* head key is bigger than the needed one, abort *)
+move: (semiconnex Ek); rewrite {}Ho' orbC /= =>Ho'; step=>_; split=>//.
+(* k is not in the head entry *)
+apply/esym/fnd_supp; rewrite Ef supp_ins inE negb_or; apply/andP; split=>//.
+(* nor it is in the tail *)
 by apply/notin_path/path_le/all_path/O'.
 Qed.
 
+(* removing an element by key from the map, return the pointer to the new map *)
+
+(* loop invariant: *)
+(* 1. we split the list into a zipper-like structure `fml ++ [k'->v'] ++ fmr` *)
+(* 2. the ordering is respected *)
+(* 3. k is not in fml nor in the focus entry k'->v' *)
+(* the focus is needed so that we can connect the remainder of the map to it after removal *)
 Definition removeT p k : Type :=
   forall (prevcur : ptr * ptr),
     {fm}, STsep (fun h => exists fml fmr k' v',
@@ -230,7 +260,7 @@ Definition removeT p k : Type :=
 Program Definition remove x (k : K) :
   {fm}, STsep (shape x fm,
               [vfun y => shape y (rem k fm)]) :=
-  Do (let: rm := Fix (fun (go : removeT x k) '(prev, cur) =>
+  Do (let: go := Fix (fun (loop : removeT x k) '(prev, cur) =>
                       Do (if cur == null then ret tt
                           else k' <-- !cur;
                                if k == k'
@@ -242,7 +272,7 @@ Program Definition remove x (k : K) :
                                       ret tt
                                  else if ord k' k
                                       then next <-- !(cur.+2);
-                                           go (cur, next)
+                                           loop (cur, next)
                                       else ret tt))
       in
       if x == null then ret null
@@ -255,86 +285,112 @@ Program Definition remove x (k : K) :
                      ret next
                 else if ord k' k
                      then next <-- !(x.+2);
-                          rm (x, next);;
+                          go (x, next);;
                           ret x
                      else ret x).
+(* first the loop *)
+(* we don't return the pointer because it cannot change, as the head is fixed by fml *)
 Next Obligation.
+(* pull out ghost var, preconditions and heap validity *)
 move=>x k0 go _ prev cur _ [_][] _ /= [fml][fmr][k][v][-> [Ol Or][El E]][hl][_][-> Hl [_][hr][->->Hr]].
-apply: vrfV=>Vh; case: eqP.
-(* cur = null, nothing to process *)
-- move=>Ec; step=>_; rewrite {}Ec in Hr *.
-  case: (shape_null (validX Vh) Hr)=>/=->->.
-  rewrite fcats0 unitR rem_ins (negbTE E) (rem_supp El).
+(* branch on cur *)
+case: eqP=>[|/eqP] Ec.
+(* cur = null - nothing to left to process, i.e., fmr = [] *)
+- apply: vrfV=>Vh; step=>_; rewrite {}Ec in Hr *.
+  (* k is not in fml ++ (k->v) *)
+  case: (shape_null (validX Vh) Hr)=>/=->->; rewrite fcats0 unitR rem_ins (negbTE E) (rem_supp El).
   by exact: shape_seg_rcons.
-(* cur <> null *)
-move/eqP=>Ec; case: (shape_cont Ec Hr)=>k'[v'][next][hr'][Efr /all_path Or' Ehr Hr'].
-rewrite {hr Hr Vh Ec}Ehr joinA joinC.
+(* cur <> null, pull out the head entry from fmr *)
+case: (shape_cont Ec Hr)=>k'[v'][next][hr'][Efr /all_path Or' {hr Hr Ec}-> Hr']; rewrite joinA joinC.
+(* derive ordering facts *)
 move/all_path: (Or); rewrite {1}Efr; case/(path_supp_ins_inv Or')/andP=>Ho' Or''.
-step; case: eqP.
-(* k = k', element found *)
-- move=>Ek; do 4!step; rewrite !unitL /entry; do 2![step]=>_.
+(* get head key, branch on comparing it to needed one *)
+step; case: eqP=>[|/eqP] Ek.
+- (* k = k' - element is found, run the deallocations *)
+  do 4!step; rewrite !unitL; do 2![step]=>_.
+  (* pull out fml ++ (k->v) *)
   rewrite Efr -fcat_srem; last by rewrite supp_ins inE negb_or E.
+  (* drop the element in the spec *)
   rewrite rem_ins {1}Ek eq_refl rem_supp; last by rewrite Ek; apply: notin_path.
+  (* heap shape is respected *)
   rewrite joinC; apply/shape_fcat/Hr'; last by apply: shape_seg_rcons.
+  (* the ordering is respected as well *)
   rewrite (allrel_in_l (xs':=k::supp fml) _); last by apply: supp_ins.
   rewrite allrel_consl path_all //=.
   by apply/(allrel_trans (z:=k))/path_all=>//; exact: trans.
-(* k <> k' *)
-move/eqP=>Ek; case: ifP=>Ho0.
-(* ord k' k, recursive call *)
-- step.
-  apply: [gE (fcat (ins k' v' (ins k v fml)) (behd fmr))]=>//=.
-  - exists (ins k v fml), (behd fmr), k', v'; do!split=>//.
-    - rewrite (eq_all_r (s2:=k::supp fml)) /= ?Ho' /=; last by apply: supp_ins.
+(* k <> k', now branch on order comparison *)
+case: ifP=>Ho0.
+- (* k' is less than k, invoke the loop, shifting the focus to the right *)
+  step; apply: [gE (fcat (ins k' v' (ins k v fml)) (behd fmr))]=>//=.
+  - (* prove that all conditions are respected *)
+    exists (ins k v fml), (behd fmr), k', v'; do!split=>//.
+    - (* new focus comes after fml ++ old focus *)
+      rewrite (eq_all_r (s2:=k::supp fml)) /= ?Ho' /=; last by apply: supp_ins.
       by apply/sub_all/Ol=>? /trans; apply.
-    - by apply: path_all.
-    - by rewrite supp_ins inE negb_or E.
+    - (* new focus comes before the new suffix *)
+      by apply: path_all.
+    - (* the needed key is not in fml ++ old focus *)
+      by rewrite supp_ins inE negb_or E.
+    (* heap shape is respected *)
     exists (hl \+ entry prev cur k v), (entry cur next k' v' \+ hr').
-    rewrite joinC !joinA; do!split=>//; last by exists (entry cur next k' v'), hr'.
-    by rewrite -!joinA; apply: shape_seg_rcons.
+    rewrite joinC; split=>//; last by vauto.
+    by apply: shape_seg_rcons.
+  (* we can reassemble the spec because insertions of old and new foci commute *)
   case=>//= [[]] m Vm Hm; rewrite Efr.
-  rewrite fcat_inss // in Hm; first by rewrite -fcat_sins in Hm.
-  by apply: notin_path.
-(* ord k k', abort *)
+  by rewrite fcat_inss // -?fcat_sins // in Hm; apply: notin_path.
+(* k' is bigger than k, abort *)
 move: (semiconnex Ek); rewrite {}Ho0 orbC /= =>Ho0.
 step=>_; rewrite rem_supp.
-- rewrite joinC; apply: shape_fcat; first 1 last.
+- (* the shape is preserved *)
+  rewrite joinC; apply: shape_fcat; first 1 last.
   - by apply: shape_seg_rcons.
   - by rewrite Efr; apply: shape_cons=>//; apply: path_all.
+  (* ordering is preserved *)
   rewrite (allrel_in_l (xs':=k::supp fml) _); last by apply: supp_ins.
   rewrite allrel_consl Or /=.
   by apply/(allrel_trans (z:=k))=>//; exact: trans.
+(* the element wasn't found *)
 rewrite Efr supp_fcat !inE negb_or; apply/andP; split;
   rewrite supp_ins !inE negb_or; apply/andP; split=>//.
 by apply/notin_path/path_le/Or'.
 Qed.
+(* now the outer function, which mostly repeats the loop *)
+(* the first iteration is special because we don't yet have a left prefix *)
+(* to connect to the remainder if the head is removed *)
 Next Obligation.
-move=>/= x k0 [fm][]i /= H; apply: vrfV=>Vh.
-case: eqP.
-(* x = null, nothing to process *)
-- by move: H=>/[swap] ->/(shape_null Vh) [->->]; step=>_.
-(* x <> null *)
-move/eqP=>Ex {Vh}; case: (shape_cont Ex H)=>{Ex}k[v][next][h'][Ef Of Eh H']; rewrite Eh.
-step; case: eqP.
-(* k = k', element found in head position *)
-- move=>->; do 5!step; rewrite !unitL=>_.
-  rewrite Ef rem_ins eq_refl rem_supp //.
+(* pull out ghost+precondition, branch on x *)
+move=>/= x k0 [fm][]i /= H; case: eqP=>[|/eqP] Ex.
+- (* x is null, nothing to process *)
+  by apply: vrfV=>Vh; move: H; rewrite Ex =>/(shape_null Vh) [->->]; step=>_.
+(* x <> null, pull out the head entry *)
+case: (shape_cont Ex H)=>{Ex}k[v][next][h'][Ef Of Eh H']; rewrite Eh.
+(* read the key, branch on equality comparison *)
+step; case: eqP=>[->|/eqP Ek].
+- (* k = k', element found in head position, run deallocations, return new head *)
+  do 5![step]=>_; rewrite !unitL Ef rem_ins eq_refl rem_supp //.
   by apply/notin_path/all_path.
-(* k <> k' *)
-move/eqP=>Ek; case: ifP=>Ho0.
-(* ord k' k, start recursing *)
+(* k <> k', now branch on order comparison *)
+case: ifP=>Ho0.
+(* k' is less than k, start the loop with the head entry as the focus *)
 - step; apply: [stepE fm]=>/=; last by case=>//= [[]] ??; step.
+  (* invariants and shape are satisfied *)
   exists nil, (behd fm), k, v; do!split=>//.
   - by rewrite fcat_inss; [rewrite fcat0s|apply/notin_path/all_path].
-  exists Unit, (entry x next k v \+ h'); do!split; first by rewrite /entry unitL !joinA.
-  by exists (entry x next k v), h'.
-(* ord k k', abort *)
+  by exists Unit, (entry x next k v \+ h'); split=>//; [rewrite unitL | vauto].
+(* k' is bigger than k, abort *)
 move: (semiconnex Ek); rewrite {}Ho0 orbC /= =>Ho0.
-step=>_.
-rewrite -Eh rem_supp // Ef supp_ins !inE negb_or Ek /=.
+(* return the old head, invariants are preserved *)
+step=>_; rewrite -Eh rem_supp // Ef supp_ins !inE negb_or Ek /=.
 by apply/notin_path/path_le/all_path/Of.
 Qed.
 
+(* upserting (inserting or updating if the key is found) an entry into the map, return the pointer to the new map *)
+
+(* loop invariant, essentially identical to remove: *)
+(* 1. as for remove, we split the list into a zipper-like structure `fml ++ [k'->v'] ++ fmr` *)
+(* 2. the ordering is respected *)
+(* 3. k is not in fml and is less than the key k' of focus entry *)
+(* the focus is needed so that we can connect the new element to it after insertion *)
 Definition insertT p k v : Type :=
   forall (prevcur : ptr * ptr),
     {fm}, STsep (fun h => exists fml fmr k' v',
@@ -350,7 +406,7 @@ Definition insertT p k v : Type :=
 Program Definition insert x (k : K) (v : V) :
   {fm}, STsep (shape x fm,
               [vfun y => shape y (ins k v fm)]) :=
-  Do (let: ns := Fix (fun (go : insertT x k v) '(prev, cur) =>
+  Do (let: go := Fix (fun (loop : insertT x k v) '(prev, cur) =>
                       Do (if cur == null
                             then new <-- allocb k 3;
                                  new.+1 ::= v;;
@@ -363,7 +419,7 @@ Program Definition insert x (k : K) (v : V) :
                                         ret tt
                                    else if ord k' k
                                         then next <-- !(cur.+2);
-                                             go (cur, next)
+                                             loop (cur, next)
                                         else new <-- allocb k 3;
                                              new.+1 ::= v;;
                                              new.+2 ::= cur;;
@@ -381,32 +437,38 @@ Program Definition insert x (k : K) (v : V) :
                     ret x
                else if ord k' k
                     then next <-- !(x.+2);
-                         ns (x, next);;
+                         go (x, next);;
                          ret x
                     else new <-- allocb k 3;
                          new.+1 ::= v;;
                          new.+2 ::= x;;
                          ret new).
+(* first the loop *)
+(* we don't return the pointer because it cannot change, as the head is fixed by fml *)
 Next Obligation.
-move=>x k0 v0 go _ prev cur _ [_][] _ /= [fml][fmr][k][v][-> [Ol Or][El Ho0]][hl][_][-> Hl [_][hr][->-> Hr]].
-apply: vrfV=>Vh.
-case: eqP.
-(* cur = null, insert as the last element *)
-- move=>Ec; rewrite {}Ec in Hr.
+(* pull out ghost var+preconditions *)
+move=>x k0 v0 loop _ prev cur _ [_][] _ /= [fml][fmr][k][v][-> [Ol Or][El Ho0]][hl][_][-> Hl [_][hr][->-> Hr]].
+(* branch on cur *)
+case: eqP=>[|/eqP] Ec.
+- (* cur = null, insert as the last element *)
+  rewrite {}Ec in Hr; apply: vrfV=>Vh.
   step=>p; rewrite ptrA unitR; do 2!step; rewrite joinC; do 2![step]=>_.
+  (* fmr is empty *)
   case: (shape_null (validX Vh) Hr)=>/=->->.
-  rewrite fcats0 unitR.
-  apply: shape_seg_rcons; last by apply: shape_seg_rcons.
+  rewrite fcats0 unitR [X in _ \+ entry _ _ _ _ \+ X]joinA.
+  (* shape and ordering invariants are satisfied *)
+  apply/shape_seg_rcons/shape_seg_rcons=>//.
   rewrite (eq_all_r (s2:=k::supp fml)) /= ?Ho0 /=; last by apply: supp_ins.
   by apply/sub_all/Ol=>? /trans; apply.
-(* cur <> null *)
-move/eqP=>Ec; case: (shape_cont Ec Hr)=>k'[v'][next][hr'][Efr Or' Ehr Hr'].
-rewrite {hr Hr Vh Ec}Ehr joinA joinC.
+(* cur <> null, pull out the head entry from fmr *)
+case: (shape_cont Ec Hr)=>k'[v'][next][hr'][Efr Or' {hr Hr Ec}-> Hr']; rewrite joinA joinC.
+(* derive ordering facts *)
 move/all_path: (Or); rewrite {1}Efr; case/(path_supp_ins_inv (all_path Or'))/andP=>Ho' /(path_all (@trans _)) Or''.
-step; case: eqP.
-(* k = k', exact key found, update *)
-- move=>Ek; do 2![step]=>_.
-  rewrite Efr -fcat_sins ins_ins -Ek eq_refl joinC.
+(* get new key, branch on equality comparison *)
+step; case: eqP=>[|/eqP] Ek.
+- (* k = k', update the value at this position *)
+  do 2![step]=>_; rewrite Efr -fcat_sins ins_ins -Ek eq_refl joinC.
+  (* invariants are preserved as the key didn't change *)
   apply: shape_fcat; first 1 last.
   - by apply: shape_seg_rcons.
   - by apply: shape_cons=>//; rewrite Ek.
@@ -415,29 +477,36 @@ step; case: eqP.
   rewrite allrel_consl allrel_consr /= Ho0 Or'' /=; apply/andP; split.
   - by apply/sub_all/Ol=>? /trans; apply.
   by apply: (allrel_trans (z:=k))=>//; exact: trans.
-(* k <> k' *)
-move/eqP=>Ek; case: ifP=>Ho'0.
-(* ord k' k, recursive call *)
-- step.
-  apply/[gE (fcat (ins k' v' (ins k v fml)) (behd fmr))]=>/=.
-  - exists (ins k v fml), (behd fmr), k', v'; do!split=>//.
-    - rewrite (eq_all_r (s2:=k::supp fml)) /= ?Ho' /=; last by apply: supp_ins.
+(* k <> k', now branch on order comparison *)
+case: ifP=>Ho'0.
+(* k' is less than k, invoke the loop, shifting the focus to the right *)
+- step; apply/[gE (fcat (ins k' v' (ins k v fml)) (behd fmr))]=>/=.
+  - (* prove that all conditions are respected *)
+    exists (ins k v fml), (behd fmr), k', v'; do!split=>//.
+    - (* new focus comes after fml ++ old focus *)
+      rewrite (eq_all_r (s2:=k::supp fml)) /= ?Ho' /=; last by apply: supp_ins.
       by apply/sub_all/Ol=>? /trans; apply.
-    - rewrite supp_ins inE negb_or andbC El /=.
+    - (* the needed key is not in fml ++ old focus *)
+      rewrite supp_ins inE negb_or andbC El /=.
       by case: ordP Ho0.
+    (* heap shape is respected *)
     exists (hl \+ entry prev cur k v), (entry cur next k' v' \+ hr').
-    rewrite joinC !joinA; do!split=>//; last by exists (entry cur next k' v'), hr'.
-    by rewrite -!joinA; apply: shape_seg_rcons.
-  case=>// [[]] m _ Hm; rewrite Efr.
+    by rewrite joinC; split=>//; [apply: shape_seg_rcons | vauto].
+  (* we can reassemble the spec because insertions of old and new foci commute *)
+  case=>//= [[]] m _ Hm; rewrite Efr.
   rewrite fcat_inss // in Hm; first by rewrite -fcat_sins in Hm.
   by apply/notin_path/all_path.
-(* ord k k', insert *)
+(* k' is bigger than k, insert at this position *)
 move: (semiconnex Ek); rewrite {}Ho'0 orbC /= =>Ho0'.
+(* run the allocation and assignments *)
 step=>new; rewrite ptrA unitR; do 2!step; rewrite joinA joinC; do 2![step]=>_.
 rewrite Efr -fcat_sins; apply: shape_fcat; first 1 last.
-- by apply: shape_seg_rcons.
-- rewrite -!joinA; apply: shape_cons; last by apply: shape_cons.
+- (* shape is respected for the prefix fml ++ old focus *)
+  by apply: shape_seg_rcons.
+- (* shape is satisfed for new element + suffix *)
+  rewrite [X in X \+ (entry _ _ _ _ \+ _)]joinA; apply/shape_cons/shape_cons=>//.
   by apply/path_all/path_supp_ins=>//; apply/path_le/all_path/Or'.
+(* ordering is respected *)
 rewrite (allrel_in_l (xs':=k::supp fml) _); last by apply: supp_ins.
 rewrite (allrel_in_r (ys':=k0::k'::supp (behd fmr)) _ _); last first.
 - by move=>?; rewrite ?(supp_ins,inE).
@@ -446,36 +515,44 @@ rewrite allrel_consl !allrel_consr /= Ho0 Ho' Or'' /=; apply/and3P; split.
 - by apply/sub_all/Ol=>? /trans; apply.
 by apply: (allrel_trans (z:=k))=>//; exact: trans.
 Qed.
+(* now the outer function, which mostly repeats the loop *)
+(* the first iteration is special because we don't yet have a left prefix *)
+(* to connect to the new element if it inserted at the head position *)
 Next Obligation.
-move=>/= x k0 v0 [fm][]h /= H; apply: vrfV=>Vh.
-case: eqP.
-(* x = null, insert as the only element *)
-- move: H=>/[swap] ->/(shape_null Vh) [->->].
+(* pull out ghost+precondition, branch on x *)
+move=>/= x k0 v0 [fm][]h /= H; case: eqP=>[|/eqP] Ex.
+- (* x = null, insert as the only element, heap and spec are empty *)
+  apply: vrfV=>Vh; move: H; rewrite Ex=>/(shape_null Vh) [->->].
+  (* run *)
   step=>p; rewrite ptrA !unitR; do 3![step]=>_.
-  by exists null, Unit; rewrite unitR.
-(* x <> null *)
-move/eqP=>Ex; case: (shape_cont Ex H)=>{Ex}k[v][next][h'][Ef Of -> H'].
-step; case: eqP.
-(* k = k', exact key found in head position, update *)
-- move=>->; do 2![step]=>_.
-  rewrite Ef ins_ins eq_refl.
+  by exists null, Unit; rewrite unitR joinA.
+(* x <> null, pull out the head entry *)
+case: (shape_cont Ex H)=>{Ex}k[v][next][h'][Ef Of {h H}-> H].
+(* read the head key, branch on equality comparison *)
+step; case: eqP=>[->|/eqP Ek].
+- (* k = k', exact key found in head position, update the head value *)
+  do 2![step]=>_; rewrite Ef ins_ins eq_refl.
   by apply: shape_cons.
-(* k <> k' *)
-move/eqP=>Ek; case: ifP=>Ho0.
-(* ord k' k, start recursing *)
-- step; apply: [stepE fm]=>/=; last by case=>// [[]] /= ??; step.
+(* k <> k', now branch on order comparison *)
+case: ifP=>Ho0.
+- (* k' is less than k, run the loop with the head entry as the focus *)
+  step; apply: [stepE fm]=>/=; last by case=>// [[]] /= ??; step.
+  (* invariants are respected *)
   exists nil, (behd fm), k, v; do!split=>//.
   - by rewrite fcat_inss; [rewrite fcat0s|apply/notin_path/all_path].
-  exists Unit, (entry x next k v \+ h'); do!split; first by rewrite /entry unitL !joinA.
-  by exists (entry x next k v), h'.
-(* ord k k', insert *)
+  by exists Unit, (entry x next k v \+ h'); split=>//; [rewrite unitL | vauto].
+(* k' is bigger than k, insert after the head *)
 move: (semiconnex Ek); rewrite {}Ho0 orbC /= =>Ho0.
+(* run allocation and assignments, return the old head *)
 step=>q; rewrite ptrA unitR; do 3![step]=>_.
-rewrite Ef -!joinA; apply: shape_cons; last by apply: shape_cons.
+(* invariants are preserved *)
+rewrite Ef [X in X \+ (entry _ _ _ _ \+ _)]joinA; apply/shape_cons/shape_cons=>//.
 by apply/path_all/path_supp_ins=>//; apply/path_le/all_path/Of.
 Qed.
 
-Definition AssocList := KVmap.make null (*shapeD shape_invert*) new free insert remove lookup.
+(* ordered association list is a KV map *)
+
+Definition AssocList := KVmap.make null new free insert remove lookup.
 
 End AssocList.
 End AssocList.
